A bunch of finished and unfinished axiom proofs added

src/Minimalistic.v
@@ -1,6 +1,59 @@
 Require Import FCF.
 Require Import Asymptotic.
+Require Import Admissibility.
 Require Import Tactics.
+Require Import FrapTactics.
+Require Import splitVector.
+Require Import Coq.Classes.Morphisms.
+
+Section TODO.
+  Lemma maxRat_eq : forall r, maxRat r r = r.
+    intros.
+    unfold maxRat.
+    cases (bleRat r r); trivial.
+  Qed.
+
+  Lemma minRat_eq : forall r, minRat r r = r.
+    intros.
+    unfold minRat.
+    cases (bleRat r r); trivial.
+  Qed.
+
+  Lemma ratDistance_0 : forall r, ratDistance r r == 0.
+    intros.
+    unfold ratDistance.
+    rewrite maxRat_eq.
+    rewrite minRat_eq.
+    apply ratSubtract_0.
+    reflexivity.
+  Qed.
+
+  Global Instance Proper_negligible : Proper (pointwise_relation nat eqRat ==> iff) negligible.
+  Proof.
+    cbv [pointwise_relation Proper respectful].
+    intros.
+    split; eauto 10 using negligible_eq.
+    intro.
+    eapply negligible_eq.
+    eassumption.
+    symmetry.
+    eauto.
+  Qed.
+
+  Global Instance Proper_negligible_le : Proper (pointwise_relation nat leRat ==> Basics.flip Basics.impl) negligible.
+  Proof.
+    cbv [pointwise_relation Proper respectful].
+    intros.
+    intro.
+    eauto using negligible_le.
+  Qed.
+
+  Lemma negligible_0 : negligible (fun _ => 0).
+    eapply negligible_le with (f1 := fun n => 0 / expnat 2 n).
+    reflexivity.
+    apply negligible_const_num.
+  Qed.
+End TODO.
 
 Section Language.
   Context {base_type : Set} {interp_base_type:base_type->Set}.
@@ -12,6 +65,8 @@ Section Language.
     | Type_base t => interp_base_type t
     | Type_arrow dom cod => interp_type dom -> interp_type cod
     end.
+
+  (* interp term takes in eta, comp_interp_term passes in eta , term should include nat -> *)
 
   Context {message list_message rand : base_type}.
   Inductive term : type -> Type :=
@@ -83,7 +138,111 @@ Section CompInterp.
       (* TODO: insert bounds on coputational complexity of [adv] and [dst] here *)
       let game eta e := universal_security_game l adv dst eta e in
       negligible (fun eta => | Pr[game eta a] -  Pr[game eta b] | ).
-End CompInterp.
+
+  Global Instance Reflexive_indist {t} : Reflexive (@indist t).
+  Proof.
+    cbv [Reflexive indist]; setoid_rewrite ratDistance_0; eauto using negligible_0.
+  Qed.
+
+  Print Reflexive.
+  Print Symmetric.
+
+  Global Instance Symmetric_indist {t} : Symmetric (@indist t).
+  Proof.
+    cbv [Symmetric indist]; intros; setoid_rewrite ratDistance_comm; eauto.
+  Qed.
+
+  Global Instance Transitive_indist {t} : Transitive (@indist t).
+  Proof.
+    cbv [Transitive indist]; intros; setoid_rewrite ratTriangleInequality; eauto using negligible_plus.
+  Qed.
+
+        (* dst : forall t : type base_type, nat -> list bool -> interp_type interp_base_type t -> bool, *)
+
+  Lemma not_indist_const {t} (x y : interp_type interp_base_type t) (tEqDec:forall x y : interp_type interp_base_type t, {x=y}+{x<>y}) (typeDec : forall x y : type base_type, {x=y}+{x<>y}) (H:x <> y) : ~indist (Term_const x) (Term_const y).
+  Proof.
+    cbv [indist].
+    intro X.
+    specialize (X id (fun _ _ _ => nil)
+                  ((fun t' => match typeDec t t' with
+                           | left pfeq => fun _ _ x' => ltac:(
+                                                      rewrite <- pfeq in x'; exact (if tEqDec x x' then true else false))
+                           | right pfne => fun _ _ _ => false
+                           end))).
+
+    cbv [universal_security_game comp_interp_term interp_term] in X.
+    destruct (typeDec t t) in X; [|congruence].
+    cbv [eq_rec_r eq_rec eq_rect eq_sym] in X.
+    replace e with (eq_refl:t=t) in X by admit.
+
+    destruct (tEqDec x x) in X; [|congruence].
+    destruct (tEqDec x y) in X; [congruence|].
+    cbv[negligible] in X.
+    specialize (X 1%nat).
+    destruct X as [n' X].
+    specialize (X (1+n')%nat).
+    assert (nz (1+n')) by (constructor; omega).
+    specialize (X H0).
+    assert (1 + n' > n') by omega.
+    specialize (X H1).
+    apply X; clear X.
+
+    lazymatch goal with
+      |- context [ Pr [?C] ] =>
+      let H := fresh "H" in
+      assert (Pr [C] == 1) as H;
+        [|rewrite H; clear H]
+    end.
+    {
+      fcf_irr_l; fcf_well_formed; fcf_irr_l; fcf_well_formed; fcf_compute.
+    }
+
+  lazymatch goal with
+    |- context [ Pr [?C] ] =>
+    let H := fresh "H" in
+    assert (Pr [C] == 0) as H;
+    [|rewrite H; clear H]
+  end.
+    {
+      fcf_irr_l; fcf_well_formed; fcf_irr_l; fcf_well_formed; fcf_compute.
+    }
+    {
+      lazymatch goal with |- ?a <= ?b => change (a <= 1) end.
+      apply rat_le_1.
+      apply expnat_ge_1.
+      omega.
+    }
+  Admitted.
+    (* fcf_compute. *)
+    (* Unset Printing Notations. *)
+    (* Show. *)
+
+    (* fcf_simp. *)
+
+    (* SearchAbout Rat. *)
+
+    (* SearchAbout Rat refl. *)
+
+    (* fcf_irr_r. *)
+    (* Print RatRel. *)
+    (* constructor; eauto. *)
+  (* Context (KeyGen : forall n, term rand -> Key n). *)
+  (* Context (Encrypt : forall n, Key n -> Plaintext n -> term rand -> Ciphertext n). *)
+  (* Context (Decrypt : forall n, Key n -> Ciphertext n -> Plaintext n). *)
+
+  (* Context (admissible_A1: pred_oc_fam). *)
+  (* Context (admissible_A2: pred_oc_func_2_fam). *)
+
+  (* Lemma indist_encrypt : *)
+  (*   forall n (p0 p1 : term Plaintext n) (n0 n1 : nat), *)
+  (*     n0 <> n1 -> *)
+  (*     indist (Term_app (Term_const (Encrypt n)) ((Term_const (KeyGen n))  p0) *)
+  (* Lemma indist_refl {t} (x:term t) : indist x x. *)
+(* End SymbolicProof. *)
+
+
+(** proving soundness of symbolic axioms *)
+  End CompInterp.
 
 Section SymbolicProof.
   Context {base_type : Set} {interp_base_type : base_type -> Set}.
@@ -106,10 +265,85 @@ Definition if_then_else {t : type base_type}
   : interp_type interp_base_type (Type_arrow (type_base BaseType_bool) (Type_arrow t (Type_arrow t t)))
   := fun (b : bool) (x y : interp_type interp_base_type t) => if b then x else y.
 
-(** proving soundness of symbolic axioms *)
+Definition image_relation {T} (R:T->T->Prop) {A} (f:A->T) := fun x y => R (f x) (f y).
+Global Instance Equivalence_image_relation {T R} {Equivalence_R:Equivalence R} {A} (f:A->T) :
+  Equivalence (image_relation R f).
+Admitted.
+
+Definition Distribution_eq {A} := pointwise_relation A eqRat.
+Global Instance Equivalence_Distribution_eq {A} : Equivalence (@Distribution_eq A).
+Admitted.
+
+Definition Comp_eq {A} := image_relation Distribution_eq (@evalDist A).
+Check (_:Equivalence Comp_eq).
+
+Global Instance Proper_evalDist {A} : Proper (Comp_eq ==> Distribution_eq) (@evalDist A).
+Proof. exact (fun _ _ => id). Qed.
+
+Global Instance Proper_getSupport {A} : Proper (Comp_eq ==> (@Permutation.Permutation _)) (@getSupport A).
+Proof. intros ???; eapply evalDist_getSupport_perm_id; assumption. Qed.
+
+Global Instance Proper_sumList {A:Set} : Proper ((@Permutation.Permutation A) ==> (Logic.eq ==> eqRat) ==> eqRat) (@sumList A).
+Proof.
+Admitted.
+
+Global Instance Proper_Bind {A B} : Proper (Comp_eq ==> (Logic.eq==>Comp_eq) ==> Comp_eq) (@Bind A B).
+Proof.
+  intros ?? H ?? G ?. simpl evalDist.
+
+  (* TODO: find out why setoid rewrite does not do this *)
+  etransitivity; [|reflexivity].
+  eapply Proper_sumList.
+  eapply Proper_getSupport.
+  eassumption.
+  intros ? ? ?; subst.
+  f_equiv.
+  { eapply Proper_evalDist. assumption. }
+  { eapply Proper_evalDist. eapply G. reflexivity. }
+Qed.
+
+
+Lemma Rnd_split_equiv n1 n2 : Comp_eq
+    (x <-$ { 0 , 1 }^ n1 + n2; ret splitVector n1 n2 x)
+    (x1 <-$ { 0 , 1 }^ n1; x2 <-$ { 0 , 1 }^ n2; ret (x1, x2)).
+Proof. intro z. eapply Rnd_split_equiv. Qed.
+
+Lemma eq_impl_negligible : forall A (x y : nat -> Comp A), pointwise_relation _ Comp_eq x y -> forall t, negligible (fun eta : nat => | evalDist (x eta) t - evalDist (y eta) t|).
+  Admitted.
+
+Lemma Comp_eq_bool (x y:Comp bool) :
+ well_formed_comp x
+ -> well_formed_comp y
+  -> Pr [x] == Pr[y]
+  -> Comp_eq x y.
+  intros.
+  intro b.
+  destruct b; trivial.
+  rewrite !evalDist_complement; trivial.
+  f_equiv; trivial.
+Qed.
+
+Lemma Comp_eq_evalDist A (x y:Comp A) :
+ well_formed_comp x
+ -> well_formed_comp y
+  -> (forall c, evalDist x c == evalDist y c)
+  -> Comp_eq x y.
+  intros.
+  intro b.
+  apply H1.
+Qed.
+(* Lemma Comp_eq_impl_evalDist A (x y : Comp A): *)
+(*   Comp_eq x y -> *)
+(*   evalDist *)
+Print Distribution.
 
 Axiom random_size : nat -> nat.
 Goal False.
+
+  (* pose_proof (forall t (x : term t), indist x x) as H. *)
+
+  (* pose proof (fun A B => indist_if_then_else_rand_l (bool:=BaseType_bool) (@indist random_size) (fun _ => Term_const if_then_else) A B) as H. *)
+
   pose proof (fun A B => indist_if_then_else_rand_l (bool:=BaseType_bool) (@indist random_size) (fun _ => Term_const if_then_else) A B) as H.
   match type of H with ?A -> ?C => assert A as HA; [clear H|specialize(H HA);clear HA] end.
 
@@ -121,20 +355,53 @@ Goal False.
   cbv [rand_end indist universal_security_game comp_interp_term interp_term]. (* to monadic probability notation *)
   intros.
   pose proof negligible_const_num 1.
-  eapply negligible_le; [intro eta;etransitivity|..]. {
-    setoid_rewrite evalDist_commute.
-    rewrite !mult_succ_l.
-    generalize (random_size eta) as D; intro D.
-    eapply evalDist_bind_distance.
-    { eapply well_formed_Rnd. }
-    { intros. reflexivity. }
-    { intros evil_rand_tape probe Hevil_rand_tape.
-      set (dst (Type_base BaseType_message) eta (Vector.to_list evil_rand_tape)) as attack.
-      SearchAbout (Rnd (_ + _)).
-      SearchAbout (Bind (Ret _ _) _).
-      SearchAbout Bind Ret.
-      SearchAbout evalDist Bind.
+  apply eq_impl_negligible.
+  intros eta.
+  apply Comp_eq_bool.
+  fcf_well_formed.
+  fcf_well_formed.
+  dist_swap_l.
+  dist_swap_r.
+  fcf_skip.
+  generalize (random_size eta) as D; intro D.
 
+  assert (Pr [c <-$ (d <-$ (a <-$ { 0 , 1 }^ x * D + D; ret (splitVector (x * D) D a)); ret snd d);
+              ret dst (Type_base BaseType_message) eta (Vector.to_list x0) (Vector.to_list c) ] ==
+          Pr [c <-$ (d <-$ (a <-$ { 0 , 1 }^ y * D + D; ret (splitVector (y * D) D a)); ret snd d);
+              ret dst (Type_base BaseType_message) eta (Vector.to_list x0) (Vector.to_list c) ] ).
+  {
+    fcf_skip.
+    match goal with |- evalDist ?C1 ?x == evalDist ?C2 ?x => generalize x; change (Comp_eq C1 C2) end.
+    setoid_rewrite Rnd_split_equiv.
+    apply Comp_eq_evalDist.
+    {
+      fcf_well_formed.
+    }
+    {
+      fcf_well_formed.
+    }
+    {
+      intros.
+      fcf_inline_first.
+      fcf_at fcf_inline fcf_left 1%nat.
+      fcf_at fcf_inline fcf_right 1%nat.
+      fcf_swap fcf_left.
+      fcf_swap fcf_right.
+      fcf_skip.
+      fcf_at fcf_ret fcf_left 1%nat.
+      fcf_at fcf_ret fcf_right 1%nat.
+      cbv [snd].
+      fcf_irr_l.
+      {
+        fcf_well_formed.
+      }
+      fcf_irr_r.
+      {
+        fcf_well_formed.
+      }
+    }
+  }
+  Admitted.
 
 
 (* 2 subgoals, subgoal 1 (ID 34) *)
@@ -163,7 +430,7 @@ Goal False.
   (* This probably could be proven in this form -- the argument is that the two subsequences of the good random tape that are given to [dst] are non-overlapping. *)
 
   
-  simpl. (* to raw probability equations *)
+  (* simpl. (* to raw probability equations *) *)
   
 (* 2 subgoals, subgoal 1 (ID 141) *)
   
